Update source_to_flat proof for changed sig semantics
Previously the proof relied on the compiler's global variable mapping's
domain being the same as the source semantics'. This is no longer true
now that the source semantics is restricted by the signature (but the
compiler's mapping isn't, because that would require the compiler to
track the signatures for no reason). Now the theorem just relies on the
domains being the same for top-level bindings only.

Some cheats remain in what should be fairly easy places

compiler/backend/proofs/source_to_flatProofScript.sml
@@ -603,7 +603,7 @@ val (env_all_rel_rules, env_all_rel_ind, env_all_rel_cases) = Hol_reln `
     env_rel genv env_v_local env'
     ⇒
     env_all_rel genv map
-      <| c := env.c; v := nsAppend env_v_local env.v |>
+      <| c := env.c; v := nsAppend env_v_local env.v; s := env.s |>
       <| c := FDOM genv.c; v := env'; exh_pat := F; check_ctor := T |>
       locals)`;
 
@@ -1146,7 +1146,7 @@ val lookup_build_rec_env_lem = Q.prove (
   full_simp_tac(srw_ss())[]);
 
 val sem_env_eq_lemma = Q.prove (
-  `!(env:'a sem_env) x. (env with v := x) = <| v := x; c := env.c |>`,
+  `!(env:'a sem_env) x. (env with v := x) = <| v := x; c := env.c; s := env.s |>`,
   rw [] >>
   rw [sem_env_component_equality]);
 
@@ -1992,7 +1992,7 @@ val compile_exp_correct' = Q.prove (
     first_x_assum match_mp_tac >> simp[] >>
     full_simp_tac(srw_ss())[env_all_rel_cases] >>
     rw [] >>
-    qexists_tac `build_rec_env funs <|v := nsAppend (alist_to_ns l) env'.v; c := env'.c|> (alist_to_ns l)` >>
+    qexists_tac `build_rec_env funs <|v := nsAppend (alist_to_ns l) env'.v; c := env'.c; s := env'.s|> (alist_to_ns l)` >>
     qexists_tac `env'` >>
     rw [semanticPrimitivesPropsTheory.build_rec_env_merge,build_rec_env_merge]
     >- (
@@ -2192,31 +2192,47 @@ val compile_decs_num_bindings = Q.prove(
   pairarg_tac >>
   fs []);
 
+val same_top_binds_def = Define `
+  same_top_binds ns1 ns2 ⇔
+    (!x. nsLookup ns1 (Short x) = NONE ⇔ nsLookup ns2 (Short x) = NONE) ∧
+    (!mn. nsLookupMod ns1 [mn] = NONE ⇔ nsLookupMod ns2 [mn] = NONE)`;
+
 val env_domain_eq_def = Define `
   env_domain_eq (var_map : source_to_flat$environment) (env : 'a sem_env)⇔
-    nsDom var_map.v = nsDom env.v ∧
-    nsDomMod var_map.v = nsDomMod env.v ∧
-    nsDom var_map.c = nsDom env.c ∧
-    nsDomMod var_map.c = nsDomMod env.c`;
+    same_top_binds var_map.v env.v ∧
+    same_top_binds var_map.c env.c`;
 
-val env_domain_eq_append = Q.prove (
+Theorem env_domain_eq_append
   `env_domain_eq env1 env1' ∧
    env_domain_eq env2 env2'
    ⇒
-   env_domain_eq (extend_env env1 env2) (extend_dec_env env1' env2')`,
-  rw [env_domain_eq_def, extend_env_def, extend_dec_env_def,nsLookupMod_nsAppend_some,
-      nsLookup_nsAppend_some, nsLookup_nsDom, namespaceTheory.nsDomMod_def,
-      EXTENSION, GSPECIFICATION, EXISTS_PROD] >>
-  metis_tac [option_nchotomy, NOT_SOME_NONE, pair_CASES]);
+   env_domain_eq (extend_env env1 env2) (extend_dec_env env1' env2')`
+ (rw [env_domain_eq_def, extend_env_def, extend_dec_env_def,nsLookupMod_nsAppend_none,
+      nsLookup_nsAppend_none, nsLookup_nsDom, namespaceTheory.nsDomMod_def,
+      EXTENSION, GSPECIFICATION, EXISTS_PROD, same_top_binds_def,
+      namespaceTheory.id_to_mods_def]
+  >- (
+    EQ_TAC >> rw []
+    >- metis_tac []
+    >- (Cases_on `p1` >> fs [] >> rw [] >> metis_tac [NOT_SOME_NONE])
+    >- metis_tac []
+    >- (Cases_on `p1` >> fs [] >> rw [] >> metis_tac [NOT_SOME_NONE]))
+  >- (
+    EQ_TAC >> rw []
+    >- metis_tac []
+    >- (Cases_on `p1` >> fs [] >> rw [] >> metis_tac [NOT_SOME_NONE])
+    >- metis_tac []
+    >- (Cases_on `p1` >> fs [] >> rw [] >> metis_tac [NOT_SOME_NONE])));
 
-val global_env_inv_append = Q.prove (
+Theorem global_env_inv_append
   `!genv var_map1 var_map2 env1 env2.
     env_domain_eq var_map1 env1 ∧
     global_env_inv genv var_map1 {} env1 ∧
     global_env_inv genv var_map2 {} env2
     ⇒
-    global_env_inv genv (extend_env var_map1 var_map2) {} (extend_dec_env env1 env2)`,
-  rw [env_domain_eq_def, v_rel_eqns, nsLookup_nsAppend_some, extend_env_def, extend_dec_env_def] >>
+    global_env_inv genv (extend_env var_map1 var_map2) {} (extend_dec_env env1 env2)`
+ (rw [env_domain_eq_def, same_top_binds_def, v_rel_eqns, nsLookup_nsAppend_some,
+      extend_env_def, extend_dec_env_def, get_shorts_def, get_first_mods_def] >>
   first_x_assum drule >>
   rw []
   >- rw []
@@ -2227,12 +2243,12 @@ val global_env_inv_append = Q.prove (
     rw [] >>
     disj2_tac >>
     rw []
+    >- (Cases_on `x` >> fs [namespaceTheory.id_to_mods_def, nsLookupLong_none])
     >- (
-      fs [EXTENSION, namespaceTheory.nsDom_def, GSPECIFICATION, UNCURRY, LAMBDA_PROD, EXISTS_PROD] >>
-      metis_tac [NOT_SOME_NONE, option_nchotomy])
-    >- (
-      fs [EXTENSION, namespaceTheory.nsDomMod_def, GSPECIFICATION, UNCURRY, LAMBDA_PROD, EXISTS_PROD] >>
-      metis_tac [NOT_SOME_NONE, option_nchotomy]))
+      Cases_on `x` >>
+      fs [namespaceTheory.id_to_mods_def, nsLookupLong_none] >>
+      Cases_on `p1` >> fs [] >> rw [] >>
+      metis_tac [nsLookupMod_none_imp, APPEND, list_distinct]))
   >- rw []
   >- (
     rw [] >>
@@ -2240,12 +2256,12 @@ val global_env_inv_append = Q.prove (
     rw [] >>
     disj2_tac >>
     rw []
+    >- (Cases_on `x` >> fs [namespaceTheory.id_to_mods_def, nsLookupLong_none])
     >- (
-      fs [EXTENSION, namespaceTheory.nsDom_def, GSPECIFICATION, UNCURRY, LAMBDA_PROD, EXISTS_PROD] >>
-      metis_tac [pair_CASES, NOT_SOME_NONE, option_nchotomy])
-    >- (
-      fs [EXTENSION, namespaceTheory.nsDomMod_def, GSPECIFICATION, UNCURRY, LAMBDA_PROD, EXISTS_PROD] >>
-      metis_tac [NOT_SOME_NONE, option_nchotomy])));
+      Cases_on `x` >>
+      fs [namespaceTheory.id_to_mods_def, nsLookupLong_none] >>
+      Cases_on `p1` >> fs [] >> rw [] >>
+      metis_tac [nsLookupMod_none_imp, APPEND, list_distinct])))
 
 val pmatch_lem =
   pmatch
@@ -2314,7 +2330,7 @@ val global_env_inv_extend = Q.prove (
       <|c := nsEmpty;
         v := alist_to_ns (alloc_defs tt (LENGTH g1) (REVERSE (MAP FST pat_env')))|>
       ∅
-      <|v := alist_to_ns pat_env; c := nsEmpty|>`,
+      <|v := alist_to_ns pat_env; c := nsEmpty; s := nsEmpty|>`,
   rw [v_rel_eqns, extend_dec_env_def, extend_env_def, nsLookup_nsAppend_some,
       nsLookup_alist_to_ns_some] >>
   rfs [Once (GSYM alookup_distinct_reverse)] >>
@@ -2867,7 +2883,8 @@ val compile_decs_correct' = Q.prove (
   simp [terminationTheory.evaluate_decs_def] >>
   conj_tac
   >- (
-    rw [compile_decs_def, evaluate_decs_def, v_rel_eqns, invariant_def, env_domain_eq_def] >>
+    rw [compile_decs_def, evaluate_decs_def, v_rel_eqns, invariant_def,
+        env_domain_eq_def, same_top_binds_def] >>
     rw [extend_dec_env_def, evaluate_decs_def, extend_env_def, empty_env_def] >>
     qexists_tac `genv` >>
     metis_tac [SUBMAP_REFL, subglobals_refl]) >>
@@ -3087,12 +3104,13 @@ val compile_decs_correct' = Q.prove (
             rw []) >>
           metis_tac [])
         >- (
-          fs [env_domain_eq_def] >>
+          fs [env_domain_eq_def, same_top_binds_def] >>
           drule (CONJUNCT1 pmatch_bindings) >>
           simp [GSYM MAP_MAP_o, fst_alloc_defs, EXTENSION] >>
           rw [MEM_MAP] >>
           imp_res_tac env_rel_dom >>
           fs [] >>
+          cheat >>
           metis_tac [FST, MEM_MAP])
         >- (
           fs [] >>
@@ -3132,7 +3150,8 @@ val compile_decs_correct' = Q.prove (
           semanticPrimitivesTheory.build_rec_env_def] >>
       qexists_tac `genv` >>
       rw [] >>
-      fs [invariant_def, v_rel_eqns, s_rel_cases, env_domain_eq_def] >>
+      fs [invariant_def, v_rel_eqns, s_rel_cases, env_domain_eq_def,
+          same_top_binds_def] >>
       metis_tac [subglobals_refl])
     >- ( (* One function *)
       fs [compile_decs_def] >>
@@ -3174,8 +3193,9 @@ val compile_decs_correct' = Q.prove (
         rw [] >>
         res_tac >>
         fs [])
-      >- rw [env_domain_eq_def, semanticPrimitivesTheory.build_rec_env_def,
-             alloc_defs_def]
+      >- (rw [env_domain_eq_def, semanticPrimitivesTheory.build_rec_env_def,
+             alloc_defs_def, same_top_binds_def] >>
+         cheat)
       >- (
         rw [v_rel_eqns, nsLookup_alist_to_ns_some,
             semanticPrimitivesTheory.build_rec_env_def, EL_LUPDATE] >>
@@ -3251,12 +3271,15 @@ val compile_decs_correct' = Q.prove (
         res_tac >>
         fs [])
       >- (
-        rw [env_domain_eq_def, semanticPrimitivesPropsTheory.build_rec_env_merge] >>
+        rw [env_domain_eq_def, same_top_binds_def,
+            semanticPrimitivesPropsTheory.build_rec_env_merge] >>
         rw [EXTENSION, GSYM MAP_MAP_o, fst_alloc_defs] >>
-        rw [MEM_MAP, EXISTS_PROD])
+        rw [MEM_MAP, EXISTS_PROD] >>
+        cheat)
       >- (
         fs [Abbr`s2`, semanticPrimitivesPropsTheory.build_rec_env_merge] >>
-        qmatch_abbrev_tac `global_env_inv <| v := g1++middle++g2; c := _ |> _ _ <| v := alist_to_ns pat_env; c := _ |>` >>
+        qmatch_abbrev_tac `global_env_inv <| v := g1++middle++g2; c := _ |> _ _
+        <| v := alist_to_ns pat_env; c := _; s := _ |>` >>
         qspecl_then [`pat_env`,
                      `<| v := g1 ⧺ middle ⧺ g2;
                          c := genv.c|>`,
@@ -3346,7 +3369,7 @@ val compile_decs_correct' = Q.prove (
       qexists_tac `genv` >>
       simp [] >>
       fs [v_rel_eqns, s_rel_cases] >>
-      rw [env_domain_eq_def, subglobals_refl]) >>
+      rw [env_domain_eq_def, same_top_binds_def, subglobals_refl]) >>
     strip_tac >>
     rename [`EVERY check_dup_ctors (td::tds)`] >>
     `?tvs tn ctors. td = (tvs, tn ,ctors)` by metis_tac [pair_CASES] >>
@@ -3391,10 +3414,12 @@ val compile_decs_correct' = Q.prove (
     >- (
       fs [env_domain_eq_def, build_tdefs_def, ADD1] >>
       ONCE_REWRITE_TAC [nsAppend_foldl] >>
-      rw [build_tdefs_no_mod, nsDom_nsAppend_flat, nsDomMod_nsAppend_flat,
+      rw [build_tdefs_no_mod, same_top_binds_def, nsDom_nsAppend_flat,
+          nsDomMod_nsAppend_flat,
           o_DEF, build_constrs_def, MAP_REVERSE, MAP_MAP_o, EXTENSION] >>
       eq_tac >>
       rw [MEM_MAP, EXISTS_PROD] >>
+      cheat >>
       metis_tac [FST])
     >- (
       fs [build_tdefs_def, v_rel_eqns] >>
@@ -3406,6 +3431,7 @@ val compile_decs_correct' = Q.prove (
         rw [Once nsAppend_foldl] >>
         rw [nsLookup_nsAppend_some])
       >- (
+        cheat >>
         fs [build_constrs_def, nsLookup_alist_to_ns_some, env_domain_eq_def] >>
         rw [Once nsAppend_foldl] >>
         rw [nsLookup_nsAppend_some] >>
@@ -3422,7 +3448,7 @@ val compile_decs_correct' = Q.prove (
     fs [evaluate_decs_def, evaluate_dec_def] >>
     qexists_tac `genv` >>
     fs [invariant_def, s_rel_cases, v_rel_eqns, extend_dec_env_def, extend_env_def,
-        empty_env_def, env_domain_eq_def] >>
+        empty_env_def, env_domain_eq_def, same_top_binds_def] >>
     metis_tac [subglobals_refl])
   >- ( (* exceptions *)
     reverse (rw [evaluate_decs_def, evaluate_dec_def]) >>
@@ -3491,7 +3517,7 @@ val compile_decs_correct' = Q.prove (
       rw [subglobals_refl] >>
       `genv = <|v := s_i1.globals; c := genv.c|>` by rw [theorem "global_env_component_equality"] >>
       metis_tac [])
-    >- rw [env_domain_eq_def]
+    >- rw [env_domain_eq_def, same_top_binds_def]
     >- rw [FLOOKUP_DEF])
   >- ( (* Module *)
     pairarg_tac >>
@@ -3511,22 +3537,26 @@ val compile_decs_correct' = Q.prove (
     qexists_tac `genv'` >>
     rw [] >>
     every_case_tac >>
+    fs [] >>
+    rw [] >>
+    pairarg_tac >>
     fs []
     >- (
-      fs [env_domain_eq_def, lift_env_def] >>
-      rw [nsDom_nsLift, nsDomMod_nsLift])
+      fs [env_domain_eq_def, lift_env_def, same_top_binds_def] >>
+      rw [nsDom_nsLift, nsDomMod_nsLift, nsLookup_nsLift, nsLookupMod_nsLift] >>
+      rw [namespaceTheory.nsLookupMod_def])
     >- (
       rw [] >>
       fs [v_rel_eqns] >>
       rw [lift_env_def, nsLookup_nsLift] >>
       CASE_TAC >>
       rw [] >>
-      fs [])
-    >- rw [])
+      fs [] >>
+      cheat))
   >- ( (* Signature *)
     rw [evaluate_decs_def] >>
     qexists_tac `genv` >>
-    rw [env_domain_eq_def, empty_env_def]
+    rw [env_domain_eq_def, empty_env_def, same_top_binds_def]
     >- metis_tac [subglobals_refl] >>
     simp [Once v_rel_cases])
   >- ( (* local *)
